examples/graph/theories/Path.v
@@ -1,4 +1,5 @@
 Require Import Data.Graph.Inductive.Graph.
+Require Import Coq.Sorting.Sorted.
 Require Import Coq.Lists.List.
 Require Import Coq.Bool.Bool.
 Require Import Helper.
@@ -71,24 +72,6 @@ Proof.
   apply path_app in H2. destruct_all.
   apply path_app. simplify'.
 Qed.
-
-(*TODO: Move to helper*)
-Ltac solve_assume := repeat(split; try(intros); try(assumption); try(reflexivity)).
-
-Ltac solve_in :=
-  match goal with
-  | [ H : _ |- In ?x (?l ++ ?r)] => apply in_or_app; solve_in
-  | [ H : _ |- In ?x ?s \/ In ?x ?s'] => first [ left; solve_in | right; solve_in ] 
-  | [ H : _ |- In ?x (?x :: ?l)] => simpl; left; reflexivity
-  | [ H : _ |- In ?x (?a :: ?l)] => simpl; right; solve_in
-  | [ H : _ |- _ ] => try(reflexivity); assumption
-end. 
-
-Ltac destruct_if :=
-  match goal with 
-    | [H: (if ?b then _ else _) = _ |- _] => destruct b
-    | [H: _ |- (if ?b then _ else _) = _ ] => destruct b
-    end. 
 
 (*If there is a path from u to v, then there is a path that contains no duplicates*)
 Lemma path_no_dups: forall g u v l,
@@ -179,16 +162,6 @@ Proof.
       apply H1. } (apply (H0 (nodeList g))). intros. unfold vIn. unfold mem. destruct_if. reflexivity.
       contradiction. apply H.
 Qed.
-(*
-Lemma in_path': forall u v l,
-  path' g u v l ->
-  vIn g u = true /\ vIn g v = true.
-Proof.
-  intros. remember g as g0. induction H; subst. split; assumption.
-  eapply edges_valid in H0. destruct_all. split. apply IHpath'. reflexivity. assumption. assumption.
-  assumption.
-Qed.
-*)
 
 (*This function finds all paths of length n from u to v*)
 Lemma paths_of_length_appear: forall g u v n l,
@@ -296,8 +269,6 @@ Proof.
       apply H1 in H3. destruct_all. exfalso. eapply H. apply H3.
 Qed. 
 
-Require Import Coq.Sorting.Sorted.
-
 (*Helper lemma for some case*)
 Lemma distance_list_some: forall l g u v n,
   StronglySorted Nat.le l ->
@@ -347,422 +318,61 @@ Proof.
   - apply seq_sorted.
 Qed. 
 
-(* Key property of shortest paths - if u -> v is a shortest path passing through w, 
-  then the length is the shortest path from u to w + the shortest path from w to v (plus 1)*)
-(*Not quite true because we count endpoints multiple times - TODO: see what is needed, come back after BFS*)
-
-(*Lemma shortest_path_transitive: forall g u v l w l' l'',
-  shortest_path g u v l ->
-  In w l ->
-  shortest_path g u w l' ->
-  shortest_path g w v l'' ->
-  length l = length l' + length l'' + 1.
-Proof.
-  intros. unfold shortest_path in *. destruct_all.
-  assert (length l < length l' + length l'' + 1 \/
-  length l > length l' + length l'' + 1 \/ length l = length l' + length l'' + 1) by omega.
-  destruct H6.
-  - apply in_split_app_fst in H0. destruct_all.
-    rewrite H0 in H. apply path_app in H. destruct H.
-    assert (length l = length x + length x0 + 1). rewrite H0. rewrite app_length.
-    simpl. omega. rewrite H9 in H6. 
-    assert (length x + length x0 < length l' + length l'') by omega. clear H6. clear H9.
-    assert (length x < length l'' \/ length x0 < length l') by omega. destruct H6.
-    + exfalso. eapply H3. apply H6. 
-  rewrite H3 in H6. inversion H. assumption.
-  rewrite H4 in H8. inversion H8. assumption. apply N.eq_dec.
-  destruct H6. assert (path_list g u v (l'' ++ w :: l') = true).
-  rewrite path_app. split; assumption. rewrite H5 in H7.
-  inversion H7. rewrite app_length. simpl. omega. assumption.
-Qed.
-
-(*Decidability of [path]*)
-
-Lemma path_equiv: forall g u v,
-  (exists l, path g u v l) <-> path_of_length g u v (length(nodeList g)) = true.
-Proof.
-  intros. split; intros.
-  - setoid_rewrite path_list_equiv in H. destruct H. apply path_shorter_than_graph_size in H.
-    destruct_all. eapply path_of_size_implies_function. apply H0. apply H.
-  - setoid_rewrite path_list_equiv. pose proof (path_of_length_implies_path _ _ _ _ H).
-    destruct_all. exists x. assumption. 
-Qed.
-
 Lemma path_dec: forall g u v,
-  {exists l, path g u v l} + {~exists l, path g u v l}.
+  {exists l, path' g u v l} + {~exists l, path' g u v l}.
 Proof.
-  intros. destruct (path_of_length g u v (length(nodeList g))) eqn : ?.
-  left. apply path_equiv; assumption.
-  right. intro. apply path_equiv in H. rewrite H in Heqb0. inversion Heqb0.
+  intros. destruct (distance g u v) eqn : D.
+  - left. apply distance_some in D. destruct_all. unfold shortest_path in H.
+    destruct_all. exists x. assumption.
+  - right. rewrite distance_none in D. intro. destruct_all. apply (D x). assumption.
 Qed.
 
-
-Definition distance (g: gr a b) (u v : Node) : option nat :=
-  if (N.eq_dec u v) then if vIn g v then (Some 0) else None else
-  fold_right (fun x acc => match paths_of_length g u v x with
-                            | nil => acc
-                            | _ => Some x
-                           end) None (seq 0 (natNodes g + 1)).
-
-(*Now we prove that this actually finds the shortest path*)
-
-(*First, a helper lemma*)
-Lemma shortest_none_helper: forall l u v,
-  (fold_right
-  (fun (x : nat) (acc : option (list Node)) =>
-   match min_weight_size_n u v x with
-   | Some l =>
-       match acc with
-       | Some l' => if lt_weight_b l l' then Some l else Some l'
-       | None => Some l
-       end
-   | None => match acc with
-             | Some l => Some l
-             | None => None
-             end
-   end) None l) = None <-> (forall x, In x l -> min_weight_size_n u v x = None).
-
-Lemma distance_none: forall g u v,
-  distance g u v = None <-> (forall l, ~path' g u v l).
+(*If there is a path between u and v, there is a shortest path between u and v*)
+Lemma shortest_path_exists: forall g u v l,
+  path' g u v l ->
+  exists l', shortest_path g u v l'.
 Proof.
-  intros. unfold distance.
-
-
-Definition shortest_wpath u v l :=
-  path' g u v l /\ forall l', path' g u v l' -> le_weight l l'.
-
-Lemma find_shortest_wpath_correct: forall u v l,
-  find_shortest_wpath u v = Some l -> shortest_wpath u v l. 
-
-
-(*
-(*Inductive and Fixpoint definitions for a path between two vertices. The Fixpoint instance proves that this is
-  decidable, and we prove their equivalence*)
-Inductive path : (gr a b) -> Node -> Node -> (list Node) -> Prop :=
-  | p_start: forall g u v, eIn g u v = true -> path g u v nil
-  | p_step: forall g u v w l, 
-     path g u w l ->
-     eIn g w v = true ->
-     path g u v (w :: l) .
-
-Fixpoint path_list (g: gr a b) (u v: Node) (l: list Node) : bool :=
-  match l with
-  | nil => eIn g u v
-  | x :: tl => eIn g x v && path_list g u x tl
-  end.
-
-Lemma path_list_equiv: forall g u v l,
-  path g u v l <-> path_list g u v l = true.
-Proof.
-  intros. split; intros.
-  - induction H.
-    + simpl. assumption.
-    + simpl. rewrite andb_true_iff. split; assumption.
-  - generalize dependent v. induction l; intros; simpl.
-    + apply p_start. simpl in H. assumption.
-    + simpl in *. rewrite andb_true_iff in H. destruct H. apply p_step. apply IHl. assumption.
-      assumption.
+  intros. destruct (distance g u v) eqn : D.
+  - apply distance_some in D. destruct_all. exists x. assumption.
+  - rewrite distance_none in D. exfalso. apply (D l). assumption.
 Qed.
 
-(*Some useful results about [path]*)
-Lemma path_app: forall g u v a l1 l2,
-  path_list g u v (l1 ++ a :: l2) = true <->
-  path_list g a v l1 = true /\ path_list g u a l2 = true.
-Proof.
-  intros. split; intros. generalize dependent v. generalize dependent l2. induction l1; intros.
-  - simpl in H. simpl. rewrite andb_true_iff in H. apply H.
-  - simpl in *. simplify'; apply IHl1 in H1; destruct H1; assumption.
-  - destruct_all. generalize dependent v. generalize dependent a0. revert l2. induction l1; intros; simpl in *;
-    simplify'.
-Qed.
-
-Lemma path_remove_cycle: forall g u v w l1 l2 l3,
-  path_list g u v (l1 ++ w :: l2 ++ w :: l3) = true ->
-  path_list g u v (l1 ++ w :: l3) = true.
-Proof.
-  intros. apply path_app in H. destruct_all. apply path_app in H0. destruct_all.
-  apply path_app. simplify'.
-Qed.
-
-(*If there is a path, then there is a path with no duplicates*)
-Lemma path_no_dups: forall g u v l,
-  path_list g u v l = true ->
-  exists l1, path_list g u v l1 = true /\ NoDup l1 /\ ~In u l1 /\  ~In v l1 /\ 
-  (forall x, In x l1 -> In x l). 
-  Proof.
-    intros. induction l using (well_founded_induction
-                       (wf_inverse_image _ nat _ (@length _)
-                          PeanoNat.Nat.lt_wf_0)).
-    destruct (NoDup_dec (N.eq_dec) l).
-    - destruct (In_dec N.eq_dec u l).
-      + eapply in_split_app_fst in i. destruct_all. clear H2. subst.
-        apply path_app in H. destruct H. specialize (H0 x). destruct H0 as [l]. 
-        rewrite app_length. simpl. assert (forall n m, n < n + S(m)) by (intros; omega). apply H0.
-        apply H. exists l. simplify'. apply N.eq_dec.
-      + destruct (In_dec N.eq_dec v l).
-        * eapply in_split_app_fst in i. destruct_all; subst. clear H2. apply path_app in H.
-          destruct H. specialize (H0 x0). destruct H0 as [l]. rewrite app_length. simpl.
-          assert (forall n m, n < m + S(n)) by (intros; omega). apply H0. apply H1. exists l.
-          simplify'. apply N.eq_dec.
-        * exists l. simplify'.
-    - rewrite no_no_dup in n. destruct_all. subst. 
-      apply path_remove_cycle in H. specialize (H0 (x0 ++ x :: x2)). destruct H0 as [l].
-      repeat(rewrite app_length; simpl). omega. apply H. exists l. simplify'. apply H5 in H4.
-      apply in_app_or in H4. destruct H4. apply in_or_app. left. apply H4. simpl in H4.
-      destruct H4. subst. solve_in. solve_in. apply N.eq_dec.
-Qed.
-
-Lemma path_implies_in_graph: forall g u v l,
-  path_list g u v l = true ->
-  vIn g u = true /\ vIn g v = true /\ (forall x, In x l -> vIn g x = true).
-Proof.
-  intros. generalize dependent v. induction l; intros; simpl in H.
-  - apply edges_valid in H. simplify'.
-  - rewrite andb_true_iff in H. destruct H. apply IHl in H0. apply edges_valid in H. crush.
-Qed. 
-*)
-
-(*We want a function to get the distance between two nodes. This is a horribly inefficient function to help do this*)
-(*A terrible function to find if a path of length <= n between two vertices exists*)
-Fixpoint path_of_length (g: gr a b) (u v : Node) (n: nat) {struct n} : bool :=
-  match n with
-  | 0 => eIn g u v
-  | S(m) => if eIn g u v then true else
-  fold_right (fun x t => if path_of_length g u x m && eIn g x v then true else t) false 
-  (nodeList g)
-  end.
-
-Lemma path_of_length_implies_path: forall g u v n,
-  path_of_length g u v n = true -> exists l, path_list g u v l = true /\ length l <= n.
-Proof.
-  intros. generalize dependent v. induction n; intros.
-  - simpl in H. exists nil. split. simpl. assumption. simpl. omega.
-  - simpl in H. destruct (eIn g u v) eqn : ?.
-    exists nil. split. simpl. assumption. simpl. omega.
-    assert (forall l, fold_right
-      (fun (x : Node) (t : bool) => if path_of_length g u x n && eIn g x v then true else t) false
-      l = true-> exists x, In x l /\ path_of_length g u x n = true /\ eIn g x v = true). {
-      intros. induction l; simpl in *.
-      * inversion H0.
-      * destruct (path_of_length g u a0 n && eIn g a0 v) eqn : ?.
-        -- exists a0. split. left. reflexivity. rewrite andb_true_iff in Heqb1. apply Heqb1.
-        -- apply IHl in H0. destruct H0. exists x. destruct H0. split. right. assumption.
-           apply H1. } 
-      apply H0 in H. clear H0. destruct H. destruct H. destruct H0. apply IHn in H0.
-      destruct H0. destruct H0. exists (x :: x0). split. simpl. rewrite andb_true_iff. crush. simpl. omega.
-Qed.
-
-Lemma path_of_size_implies_function: forall g u v l n,
-  length l <= n ->
-  path_list g u v l = true -> path_of_length g u v n = true.
-Proof.
-  intros. generalize dependent v. revert u. generalize dependent n. induction l; simpl in *; intros.
-  - destruct n. simpl. apply H0. simpl. rewrite H0. reflexivity.
-  - simplify'. destruct n. omega. assert (length l <= n) by omega. clear H.
-    simpl. destruct (eIn g u v) eqn : ?. reflexivity.
-      assert (forall a l', In a l' ->
-      path_of_length g u a n = true ->
-      eIn g a v = true ->
-      fold_right
-  (fun (x : Node) (t : bool) => if path_of_length g u x n && eIn g x v then true else t)
-  false l' = true). { intros. induction l'; simpl in *.
-  - destruct H.
-  - destruct H. subst. rewrite H3. simpl. rewrite H4. simpl. reflexivity. apply IHl' in H. 
-    destruct (path_of_length g u a2 n && eIn g a2 v). reflexivity. apply H. }
-    apply (H a0). assert (vIn g a0 = true). { apply edges_valid in H1. apply H1. } unfold vIn in H3.
-    unfold mem in H3. match goal with | [H: (if ?x then _ else _) = _  |- _] => destruct x eqn : ? end.
-    assumption. inversion H3.  apply IHl. assumption. simplify'. simplify'.
-Qed.
-
-(*If there is a path, then there is a path at most as large as the number of vertices in the graph (because
-  there is a path with no duplicates and every vertex is in the graph*)
-Lemma path_shorter_than_graph_size: forall g u v l,
-  path_list g u v l = true ->
-  exists l', path_list g u v l' = true /\ length l' <= length(nodeList g).
-Proof.
-  intros. apply path_no_dups in H. destruct_all. 
-  assert (forall a, In a x -> In a (nodeList g)). intros.
-  apply path_implies_in_graph in H. destruct_all. apply H6 in H4. unfold vIn in H4.
-  unfold mem in H4.  match goal with | [H: (if ?x then _ else _) = _  |- _] => destruct x eqn : ? end.
-  assumption. inversion H4. 
-  exists x. split. apply H. eapply NoDup_incl_length. apply H0. unfold incl. apply H4.
-Qed.
-
-Definition natNodes (g : gr a b) := (BinInt.Z.abs_nat(Graph.noNodes g)).
-
-(*By the above lemma, we can simply define distance by repeatedly checking if there is a list with 
-  the given distance*)
-Definition distance (g: gr a b) (u v : Node) : option nat :=
-  if (N.eq_dec u v) then if vIn g v then (Some 0) else None else
-  fold_right (fun x acc => if path_of_length g u v x then Some (x + 1) else acc) None (seq 0 (natNodes g + 1)).
-
-Lemma distance_none: forall g u v,
-  distance g u v = None <-> ((forall l, path_list g u v l = false) /\ u <> v) \/ vIn g v = false.
-Proof.
-  intros.  assert (A: forall l, fold_right (fun (x : nat) (acc : option nat) => 
-    if path_of_length g u v x then Some (x + 1) else acc) None l = None <->
-    (forall x, In x l -> path_of_length g u v x = false)). { intros. split; intros; induction l; simpl in *.
-    destruct H0. destruct H0. subst. destruct (path_of_length g u v x) eqn : ?. inversion H.
-    reflexivity. apply IHl. destruct (path_of_length g u v a0) eqn : ?. inversion H.
-    apply H. assumption. reflexivity. destruct (path_of_length g u v a0) eqn : ?.
-    specialize (H a0). rewrite H in Heqb0. inversion Heqb0. left. reflexivity.
-    apply IHl. intros. apply H. right. assumption. } 
-     split; intros.
-  - unfold distance in H. destruct (N.eq_dec u v). destruct (vIn g v) eqn : ?. inversion H. right. reflexivity. 
-    left. split; intros.
-    assert (forall x, In x (seq 0 (natNodes g + 1)) -> path_of_length g u v x = false). { intros.
-    eapply A.  apply H. assumption. } clear H. clear A.
-    destruct (path_list g u v l) eqn : P.
-    + apply path_shorter_than_graph_size in P. destruct P. destruct H.
-      assert (path_of_length g u v (length x) = true). eapply path_of_size_implies_function.
-      reflexivity. assumption. 
-      assert (In (length x) (seq 0 (natNodes g + 1))). apply in_seq. split. omega. simpl.
-      assert (length (nodeList g) = natNodes g). unfold natNodes. rewrite noNodes_def. 
-      unfold nodeList. unfold ulabNodes. apply map_length. omega. 
-      apply H0 in H3. rewrite H3 in H2. inversion H2.
-    + reflexivity.
-    + assumption. 
-  - unfold distance. destruct (N.eq_dec u v). destruct (vIn g v) eqn : V. subst. destruct H.
-    destruct H. contradiction. inversion H. reflexivity.
-    apply A. intros. destruct (path_of_length g u v x) eqn : ?.
-    + apply path_of_length_implies_path in Heqb0. destruct Heqb0. destruct H1. destruct H. destruct H. rewrite H in H1.
-      inversion H1. apply path_implies_in_graph in H1. destruct_all. rewrite H3 in H. inversion H.
-    + reflexivity.
-Qed.
-
-Lemma seq_pred: forall start len h t n l,
-  seq start len = (h :: t) ++ S n :: l ->
-  In n (h :: t).
-Proof.
-  intros. generalize dependent h. revert t. revert start. induction len; intros.
-  - simpl. simpl in H. inversion H.
-  - simpl in H. inversion H. subst. destruct t.
-    simpl in H2. simpl. destruct len. simpl in H2. inversion H2. simpl in H2. inversion H2. subst. left. reflexivity.
-    apply IHlen in H2. solve_in.
-Qed.
-
-Lemma seq_split: forall start len l1 x l2,
-  seq start len = l1 ++ x :: l2 ->
-  (forall y, In y l1 -> y < x) /\ (forall y, In y l2 -> y > x).
-Proof.
-  intros. generalize dependent start. revert l1. revert x. revert l2. induction len; intros; simpl in H.
-  - assert (l1 = nil). destruct l1; inversion H. subst.
-    simpl in H. inversion H.
-  - destruct l1. simpl in H. inversion H. destruct l2.
-     split; intros. destruct H0. rewrite H2 in H0. destruct H0.
-     specialize (IHlen l2 n nil (S(start))). subst. simpl in IHlen. apply IHlen in H2.
-     split; intros. destruct H0. rewrite in_seq in H0. omega.
-     inversion H; subst. specialize (IHlen l2 x l1 (S(n)) H2). split; intros. simpl in H0.
-     destruct H0. subst. assert (In x (seq (S(y)) len)). rewrite H2. solve_in. rewrite in_seq in H0.
-      omega. destruct IHlen. apply H1. assumption. apply IHlen. apply H0.
-Qed.
-
-Lemma distance_neq: forall g u v n,
-  u <> v ->
+(*Every shortest path has the same length: the distance computed by [distance]*)
+Lemma shortest_path_distance: forall g u v l n,
   distance g u v = Some n ->
-  n > 0.
+  shortest_path g u v l ->
+  length l = n.
 Proof.
-  intros. unfold distance in H0. destruct (N.eq_dec u v). subst. contradiction.
-  induction (seq 0 (natNodes g + 1)).
-  - simpl in H0. inversion H0.
-  - simpl in H0. destruct (path_of_length g u v a0) eqn : ?. inversion H0; subst; omega.
-    apply IHl. assumption.
+  intros. apply distance_some in H. destruct_all. unfold shortest_path in *.
+  destruct_all. subst. assert (forall n m, n < m \/ m < n \/ n = m) by (intros; omega).
+  specialize (H1 (length l) (length x)). destruct H1. apply H3 in H1. contradiction.
+  destruct H1. apply H2 in H1. contradiction. assumption.
 Qed.
-  
 
-(*This actually computes the shortest path*)
-Lemma distance_some: forall g u v n,
-  distance g u v = Some n <-> vIn g v = true /\
-  (((u = v /\ n = 0)) \/ (n > 0 /\ u <> v /\ (exists l, path g u v l /\ length l = (n - 1)) /\ (forall l, length l < (n - 1) -> path_list g u v l = false))).
+(*The shortest path from a vertex to itself is the trivial path*)
+Lemma distance_refl: forall g v,
+  vIn g v = true ->
+  shortest_path g v v (v :: nil).
 Proof.
-  intros. 
-  assert (forall l n, 
-  fold_right (fun (x : nat) (acc : option nat) => if path_of_length g u v x then Some (x +1) else acc) None
-  l = Some (n + 1) <-> (exists l1 l2, l = l1 ++ n :: l2 /\ (forall y, In y l1 -> path_of_length g u v y = false) /\
-  path_of_length g u v n  = true)). { intros. induction l; split; intros; simpl in *.
-  - inversion H.
-  - destruct_all. destruct x; inversion H.
-  - destruct (path_of_length g u v a0) eqn : ?. 
-    + inversion H; subst. exists nil. exists l. split. simpl. 
-      assert (a0 = n0) by omega. subst. reflexivity. split; intros.
-      destruct H0. assert (a0 = n0). omega. subst. assumption. 
-    + apply IHl in H. destruct H. exists (a0 :: x). destruct_all.
-      exists x0. split. rewrite H. simpl. reflexivity.
-      split; intros. simpl in H2. destruct H2. subst. assumption. apply H0. assumption.
-      assumption.
-  - destruct_all. destruct (path_of_length g u v a0) eqn : ?. destruct x.
-    + inversion H; subst. reflexivity. 
-    + simpl in H0. inversion H; subst. specialize (H0 n1). rewrite H0 in Heqb0. inversion Heqb0.
-      left. reflexivity.
-    + destruct x. inversion H; subst. rewrite Heqb0 in H1. inversion H1.
-      inversion H; subst. apply IHl. exists x. exists x0. simplify'. }
-  destruct (vIn g v) eqn : ?.
-   destruct (N.eq_dec u v). 
-   - unfold distance. subst. destruct (N.eq_dec v v ). rewrite Heqb0. 
-    split; intros. inversion H0. subst. split. reflexivity. left. split; reflexivity. 
-   destruct H0. destruct H1; destruct_all; subst. reflexivity. contradiction.  contradiction.
-  - split; intros. split.  reflexivity.
-    pose proof (distance_neq _ _ _ _ n0 H0). assert (exists m, m + 1 = n). {
-    exists (n - 1). omega. } destruct H2 as [m]. subst.
-    right. unfold distance in H0. destruct (N.eq_dec u v). subst. contradiction. 
-    rewrite H in H0. destruct_all. clear H. split; try(assumption). split; try(assumption).
-    apply path_of_length_implies_path in H3. split. setoid_rewrite path_list_equiv. 
-    destruct  H3. destruct H. assert (length x1 = m \/ length x1 < m) by omega. destruct H4.
-    exists x1. split. assumption. omega.  
-    destruct x. simpl in H. assert (natNodes g + 1 = S(natNodes g)) by omega. rewrite H5 in H0.
-    simpl in H0. inversion H0; subst. omega. 
-    destruct m. omega. assert (length x1 <= m) by omega. assert (A:=H). 
-    apply (path_of_size_implies_function _ _ _ _ _ H5) in H. exists x1.
-    split. assumption. rewrite H2 in H. inversion H.
-    pose proof seq_pred. eapply H6. apply H0.
-    intros.   assert (In (length l) (seq 0 (natNodes g + 1))). { rewrite in_seq.
-    assert (In m (seq 0 (natNodes g + 1))). rewrite H0. solve_in. rewrite in_seq in H4.
-    omega. } rewrite H0 in H4. apply seq_split in H0. 
-    destruct H0. apply in_app_or in H4. destruct H4. 
-    destruct (path_list g u v l) eqn : ?. eapply path_of_size_implies_function in Heqb1.
+  intros. unfold shortest_path. split. constructor. assumption.
+  intros. simpl in H0. assert (length l' = 0) by omega. destruct l'.
+  intro. inversion H2. inversion H1.
+Qed. 
 
-    rewrite (H2 (length l)) in Heqb1. inversion Heqb1.
-    assumption. omega. reflexivity. simpl in H4. destruct H4. omega.
-    apply H5 in H4. omega. destruct H0. destruct H1. destruct H1; contradiction. destruct_all.
-    assert (exists m, m + 1 = n). exists (n-1). omega. destruct H6 as [m]. subst.
-    assert (length x = m ) by omega. clear H5. unfold distance. destruct (N.eq_dec u v). subst. contradiction.
-    clear n. rewrite H. 
-    assert (m <= (natNodes g)). { assert (m <= natNodes g \/ m > natNodes g) by omega. destruct H5.
-    assumption. rewrite path_list_equiv in H3. apply path_shorter_than_graph_size in H3.
-    destruct H3. destruct H3. rewrite H4 in H3. inversion H3. unfold nodeList in H7.
-    unfold ulabNodes in H7. rewrite map_length in H7. rewrite <- noNodes_def in H7.
-    unfold natNodes in H5. omega. }
-    pose proof (in_split_app_fst _ (seq 0 (natNodes g + 1)) m Nat.eq_dec).
-    assert (In m (seq 0 (natNodes g + 1))). rewrite in_seq. omega.
-    apply H7 in H8. clear H7. destruct_all. exists x0. exists x1. split. assumption.
-    apply seq_split in H7. split; intros.
-    destruct H7. destruct (path_of_length g u v y) eqn : ?.
-    apply path_of_length_implies_path in Heqb1. destruct Heqb1.
-    destruct H11. rewrite H4 in H11. inversion H11. apply H7 in H9. omega. reflexivity.
-    eapply path_of_size_implies_function. assert (length x <= m) by omega. apply H9.
-    rewrite <- path_list_equiv. assumption.
-  - split; intros. assert (A:=H0). unfold distance in H0. destruct (N.eq_dec u v). rewrite Heqb0 in H0. inversion H0.
-     assert (n > 0). eapply distance_neq.  apply n0. apply A. assert (exists m, n = m + 1).
-      destruct n. omega. exists n. omega. destruct H2. subst. rewrite H in H0. destruct_all.
-    apply path_of_length_implies_path in H3. destruct_all.
-     apply path_implies_in_graph in H3. destruct_all. rewrite H5 in Heqb0. inversion Heqb0.
-    destruct H0. inversion H0.
+Lemma distance_of_shortest_path: forall g u v l,
+  shortest_path g u v l ->
+  distance g u v = Some (length l).
+Proof.
+  intros. destruct (distance g u v) eqn : D.
+  - eapply shortest_path_distance in D. rewrite D. reflexivity. assumption.
+  - rewrite distance_none in D. unfold shortest_path in H. destruct_all. exfalso.
+    apply (D l). assumption.
 Qed.
 
 
-Definition shortest_path g u v l :=
-  path_list g u v l = true /\ (forall l', length l' < length l -> path_list g u v l' = false). 
+End AllPaths.
 
-
-*)
-(* Weighted paths. We first define a new path definition that matches the one used in FGL code*)
-
-Inductive path': (gr a b) -> Node -> Node -> (list Node) -> Prop :=
-  | p_single: forall g v, vIn g v = true -> path' g v v (v :: nil)
-  | p_multi: forall g u v v' l,
-      path' g u v' l ->
-      eIn g v' v = true ->
-      path' g u v (v :: l).
+(** Weighted Paths **)
 
 Require Import GHC.Base.
 Require Import OrdTactic.
@@ -810,12 +420,12 @@ Qed.
 Lemma req_dec: forall x y, x == y = true -> (fun x y => x == y = true) x y. intros. assumption.
 Qed.
 
-(*TODO: figure out why ring tactic is not working*)
+(*[ring] tactic does not work for some reason*)
 Add Ring b : (SORrt real_ring) (decidable req_dec).
 
 
 (*For now, I will assume that the graph is simple (no parallel edges). Eventually, I may be able to
-  relax that restriction, and it should only matter for the path proofs*)
+  relax that restriction, and it should only matter for the path proofs (TODO: resolve)*)
 Variable g : gr a b.
 Variable Hsimple: forall u v w w', WeIn g u v w -> WeIn g u v w' -> w = w'.
 Variable HNonneg: forall u v w, WeIn g u v w -> #0 <= w = true.
@@ -990,7 +600,7 @@ Lemma path_cost_cons: forall h' h t n m,
   path_cost g (h :: h' :: t) == Some (n + m) = true.
 Proof.
   intros. remember (h' :: t) as l. simpl. rewrite Heql. rewrite <- Heql. rewrite H0. rewrite H. 
-  rewrite Base.simpl_option_some_eq. (*ring*) destruct HorderedRing.
+  rewrite Base.simpl_option_some_eq. destruct HorderedRing.
   destruct real_ring. destruct (SORrt). apply Radd_comm.
 Qed. 
 
@@ -1081,73 +691,8 @@ Proof.
         rewrite some_none_eq in H0. inversion H0. rewrite some_none_eq in H0. inversion H0.
 Qed. 
 
-(*Back to not as general version*)
-(*had paths of lenght n here*)
-
-Section Min.
-
-Variable A : Type.
-Variable lt: A -> A -> Prop.
-Variable eqb : A -> A -> Prop.
-Variable lt_dec: forall x y, {lt x y} + {~lt x y}.
-Variable eq_dec: forall x y, {eqb x y} + {~ eqb x y}.
-Variable eqb_equiv: RelationClasses.Equivalence eqb.
-Variable lt_trans: forall x y z, lt x y -> lt y z -> lt x z.
-Variable lt_neq: forall x y, lt x y -> ~eqb x y.
-Variable lt_total: forall x y, lt x y \/ eqb x y \/ lt y x.
-Variable lt_antisym: forall x y, lt x y -> ~lt y x.
-Variable lt_compat_r: forall x y z, lt x y -> eqb y z -> lt x z.
-
-(*General function for finding minimum according to a decidable lt relation TODO: move this*)
-Definition min_list (l: list A) : option A :=
-  fold_right (fun x acc => match acc with
-                           | Some y => if lt_dec x y then Some x else Some y
-                           | None => Some x
-                           end) None l.
-
-(*Proof that this actually finds the minimum*)
-Lemma min_list_empty: forall (l: list A) ,
-  min_list l = None <-> l = nil.
-Proof.
-  intros. split; intros. unfold min_list in H. destruct l. reflexivity. simpl in H.
-  destruct (fold_right
-        (fun (x : A) (acc : option A) =>
-         match acc with
-         | Some y => if lt_dec x y then Some x else Some y
-         | None => Some x
-         end) None l). destruct (lt_dec a0 a1); inversion H. inversion H. subst. simpl. reflexivity.
-Qed.
-
-Lemma min_list_in: forall (l: list A) x,
-  min_list l = Some x -> In x l.
-Proof.
-  intros. generalize dependent x. induction l; intros. simpl in H. inversion H. simpl in H.
-  destruct (min_list l) eqn : M. destruct (lt_dec a0 a1). inversion H; subst. solve_in.
-  inversion H. subst. right. apply IHl. reflexivity. inversion H; subst. solve_in.
-Qed.
-
-Lemma min_list_min: forall (l: list A) x,
-  min_list l = Some x ->  forall y, ~eqb x y -> In y l -> lt x y.
-Proof.
-  intros. generalize dependent x. induction l; intros.
-  - simpl in H. inversion H.
-  - simpl in H. destruct (min_list l) eqn : M.
-    + destruct (lt_dec a0 a1).
-      * inversion H; subst. 
-        simpl in H1. destruct H1. subst. destruct eqb_equiv. unfold RelationClasses.Reflexive in Equivalence_Reflexive.
-        specialize (Equivalence_Reflexive y). contradiction. 
-        destruct (eq_dec y a1). eapply lt_compat_r. apply l0. destruct eqb_equiv as [E1 E2 E3]. eapply E2.
-        assumption.
-        eapply lt_trans. apply l0. apply IHl. assumption. reflexivity.
-        intro. destruct eqb_equiv as [E1 E2 E3]. apply E2 in H2. contradiction.
-      * inversion H; subst. simpl in H1. destruct H1.
-        subst. specialize (lt_total x y). destruct lt_total. assumption. destruct H1. contradiction.
-        contradiction. apply IHl. assumption. reflexivity. assumption.
-   + inversion H; subst. rewrite min_list_empty in M. subst. destruct H1. subst.
-     destruct eqb_equiv as [E1 E2 E3]. pose proof (E1 y). contradiction. destruct H1.
-Qed.
-
-End Min.
+(* Now, we use the [min_list] function from Helper.v to define the notion of the shortest weight path in a
+  list of paths *)
 
 Definition lt_weight_b (l1 l2: list Node) :=
   match (path_cost g l1, path_cost g l2) with
@@ -1212,13 +757,13 @@ Proof.
   destruct (path_cost g x); destruct (path_cost g z); destruct (path_cost g y); order b.
 Qed.
 
-Definition min_weight_size_n u v n := min_list _ lt_weight lt_weight_dec (paths_of_length u v n).
+Definition min_weight_size_n g u v n := min_list _ lt_weight lt_weight_dec (paths_of_length g u v n).
 
 Definition le_weight l l' := lt_weight l l' \/ eq_weight l l'.
 
 (*Now, we will show that this really does find the minimum weight path of a given length*)
-Lemma min_weight_size_correct: forall u v n l,
-  min_weight_size_n u v n = Some l ->
+Lemma min_weight_size_correct: forall g u v n l,
+  min_weight_size_n g u v n = Some l ->
   path' g u v l /\ length l = n /\ forall l', path' g u v l' /\ length l' = n -> le_weight l l' .
 Proof.
   intros. pose proof (min_list_min _ _ _ lt_weight_dec eq_weight_dec eq_weight_equiv lt_weight_trans
@@ -1228,22 +773,6 @@ Proof.
   left. apply H0. assumption. apply paths_of_length_def. apply H1.
 Qed.
 
-Lemma path_app': forall u v w l1 l2,
-  path' g u v (l1 ++ w :: l2) <->
-  path' g w v (l1 ++ w :: nil) /\ path' g u w (w :: l2).
-Proof.
-  intros. split; intros. generalize dependent v. revert l2. induction l1; intros.
-  - simpl in H. inversion H; subst. split; simpl; assumption.
-    split. simpl. constructor. eapply edges_valid in H6. apply H6.
-    eapply p_multi. apply H5. assumption.
-  - simpl in H. simpl. inversion H; subst. destruct l1; inversion H5.
-    split. eapply p_multi. apply (IHl1 l2 v'). assumption. assumption. apply (IHl1 l2 v').
-    assumption.
-  - generalize dependent v. revert u. revert l2. induction l1; intros; destruct_all. simpl in *.
-    inversion H. subst. assumption. subst. inversion H6. simpl in *.
-    inversion H; subst. destruct l1; inversion H6.
-    eapply p_multi. apply (IHl1 l2 u v'). split; assumption. assumption.
-Qed. 
 Require Import Proofs.GHC.Base.
 (*Now we can find the shortest path for a given length. We want to show that if all the edge weights
   are nonnegative, if there is a shortest path of size > n, then there is a shortest path of size at most n*)
@@ -1253,7 +782,7 @@ Lemma path_app_strong: forall u v w l1 l2 ,
     path_cost g (l1 ++ w :: nil) == Some n = true -> 
     path_cost g (w :: l2) == Some m = true -> path_cost g (l1 ++ w :: l2) == Some (n+m) = true).
 Proof.
-  intros. assert (A:= H). apply path_app' in A. split. apply A. split. apply A.
+  intros. assert (A:= H). apply path_app in A. split. apply A. split. apply A.
   intros.  pose proof path_cost_app. pose proof path_cost_path'.
   assert (exists w', path_cost g (l1 ++ w :: l2) = Some w'). apply H3. exists u. exists v. assumption.
   destruct H4 as [w']. assert (B:=H4). assert (C :path_cost g (l1 ++ w :: l2) == Some w' = true).
@@ -1290,18 +819,7 @@ Proof.
     destruct (path_cost g l2); destruct (path_cost g l3); try(reflexivity); try( order b).
 Qed.
 
-Lemma path'_remove_cycle: forall u v w l1 l2 l3,
-  path' g u v (l1 ++ w :: l2 ++ w :: l3) ->
-  path' g u v (l1 ++ w :: l3).
-Proof.
-  intros. apply path_app' in H. destruct_all. replace (w :: l2 ++ w :: l3) with ((w :: l2) ++ w :: l3) in H0 by
-  reflexivity. apply path_app' in H0. destruct_all.
-  apply path_app'. simplify'.
-Qed.
-
-
-(*If there is a path, then there is a path with no duplicates, and this list is smaller*)
-(*A very hard theorem to prove (the le_weight part), but an important property: if there is a path,
+(*A very hard theorem to prove since [ring] doesn't work, but an important property: if there is a path,
   there is a smaller weight path with no duplicates*)
 Lemma path_no_dups_strong: forall u v l,
   path' g u v l ->
@@ -1436,7 +954,7 @@ Lemma path_no_dups_strong: forall u v l,
         -- apply N.eq_dec.
       * exists l. simplify'. unfold le_weight. right. destruct (eq_weight_equiv) as [E1 E2 E3]; apply E1.
   - rewrite no_no_dup in n. destruct_all. subst. assert (A:= H). 
-      apply path'_remove_cycle in H. specialize (H0 (x0 ++ x :: x2)). destruct H0 as [l].
+      apply path_remove_cycle in H. specialize (H0 (x0 ++ x :: x2)). destruct H0 as [l].
       repeat(rewrite app_length; simpl). omega. apply H. exists l. simplify'. apply H2 in H3.
       apply in_app_or in H3. destruct H3. apply in_or_app. left. assumption. simpl in H3.
       destruct H3. subst. solve_in. solve_in. eapply le_weight_trans. apply H4.
@@ -1457,7 +975,7 @@ Lemma path_no_dups_strong: forall u v l,
       assert (Some n' == Some (a' + b') = true). rewrite <- H3. rewrite <- H8. reflexivity.
       rewrite Base.simpl_option_some_eq in H13.
       remember (x1 ++ x :: x2) as l'. 
-      assert (C:= A). apply path_app' in C. destruct C. clear H14. 
+      assert (C:= A). apply path_app in C. destruct C. clear H14. 
       assert (exists c', path_cost g (x :: l') = Some c'). eapply path_cost_path'.
       exists u. exists x. assumption. destruct H14 as [c'].
       pose proof (@path_app_strong _ _ _ _ _ A). destruct_all. clear H16. clear H17.
@@ -1485,8 +1003,6 @@ Lemma path_no_dups_strong: forall u v l,
       rewrite Eq_sym. apply Radd_0_l. apply H25. apply rplus_eq. assumption. apply Eq_refl.
       apply N.eq_dec.
 Qed.
-
-(*Finally!!!!!*)
  
 (*If there is a path, then there is a path at most as large as the number of vertices in the graph (because
   there is a path with no duplicates and every vertex is in the graph*)
@@ -1503,8 +1019,9 @@ Proof.
   assumption.
 Qed.
 
-Definition find_shortest_wpath (u v : Node) : option (list Node) :=
-  fold_right (fun x acc => match (min_weight_size_n u v x) with
+(*Our inefficient function to find shortest paths (by iterating through all paths of length <= |V|*)
+Definition find_shortest_wpath  (u v : Node) : option (list Node) :=
+  fold_right (fun x acc => match (min_weight_size_n g u v x) with
                             | None => match acc with
                                         | None => None
                                         | Some l => Some l
@@ -1522,7 +1039,7 @@ Ltac destruct_option H':= match goal with
 Lemma shortest_none_helper: forall l u v,
   (fold_right
   (fun (x : nat) (acc : option (list Node)) =>
-   match min_weight_size_n u v x with
+   match min_weight_size_n g u v x with
    | Some l =>
        match acc with
        | Some l' => if lt_weight_b l l' then Some l else Some l'
@@ -1532,16 +1049,16 @@ Lemma shortest_none_helper: forall l u v,
              | Some l => Some l
              | None => None
              end
-   end) None l) = None <-> (forall x, In x l -> min_weight_size_n u v x = None).
+   end) None l) = None <-> (forall x, In x l -> min_weight_size_n g u v x = None).
 Proof.
   intros. 
   induction l; simpl; split; intros.
   - destruct H0.
   - reflexivity.
-  -  destruct (min_weight_size_n u v a0) eqn : M.
+  -  destruct (min_weight_size_n g u v a0) eqn : M.
     destruct ( fold_right
         (fun (x : nat) (acc : option (list Node)) =>
-         match min_weight_size_n u v x with
+         match min_weight_size_n g u v x with
          | Some l =>
              match acc with
              | Some l' => if lt_weight_b l l' then Some l else Some l'
@@ -1554,7 +1071,7 @@ Proof.
          end) None l). destruct (lt_weight_b l0 l1 ); inversion H. inversion H.
     destruct ( fold_right
         (fun (x : nat) (acc : option (list Node)) =>
-         match min_weight_size_n u v x with
+         match min_weight_size_n g u v x with
          | Some l =>
              match acc with
              | Some l' => if lt_weight_b l l' then Some l else Some l'
@@ -1565,11 +1082,11 @@ Proof.
                    | None => None
                    end
          end) None l ) eqn : H'. inversion H. destruct H0. subst. apply M. apply IHl. reflexivity. assumption.
-  - destruct (min_weight_size_n u v a0) eqn : ?.
+  - destruct (min_weight_size_n g u v a0) eqn : ?.
     rewrite H in Heqo. inversion Heqo. left. reflexivity.
     destruct (fold_right
     (fun (x : nat) (acc : option (list Node)) =>
-     match min_weight_size_n u v x with
+     match min_weight_size_n g u v x with
      | Some l0 =>
          match acc with
          | Some l' => if lt_weight_b l0 l' then Some l0 else Some l'
@@ -1582,6 +1099,7 @@ Proof.
      end) None l) eqn : ?. apply IHl. intros. apply H. right. assumption. reflexivity.
 Qed.
 
+(*[find_shortest_wpath] returns None iff v is not reachable from u*)
 Lemma find_shortest_wpath_none: forall u v,
   find_shortest_wpath u v = None <-> (forall l, ~path' g u v l).
 Proof.
@@ -1594,9 +1112,9 @@ Proof.
     assert (forall n m, Nat.le n m -> Nat.lt n (m + 1)). intros. unfold Nat.lt.
     unfold Nat.le in H4. omega. apply H4. apply H2. apply H in H4.
     unfold min_weight_size_n in H4. rewrite min_list_empty in H4.
-    pose proof (paths_of_length_appear u v (length x) x). 
+    pose proof (paths_of_length_appear g u v (length x) x). 
     rewrite H4 in H5. simpl in H5. apply H5. split. assumption. reflexivity.
-  - destruct (min_weight_size_n u v x) eqn : M.
+  - destruct (min_weight_size_n g u v x) eqn : M.
     + apply min_weight_size_correct in M. destruct_all. exfalso. apply (H l). assumption.
     + reflexivity.
 Qed.
@@ -1605,6 +1123,7 @@ Qed.
 Definition shortest_wpath u v l :=
   path' g u v l /\ forall l', path' g u v l' -> le_weight l l'.
 
+(*[find_shortest_wpath] returns a shortest path*)
 Lemma find_shortest_wpath_correct: forall u v l,
   find_shortest_wpath u v = Some l -> shortest_wpath u v l. 
 Proof.
@@ -1612,7 +1131,7 @@ Proof.
   assert (forall l' l'' u' v',
    (fold_right
       (fun (x : nat) (acc : option (list Node)) =>
-       match min_weight_size_n u' v' x with
+       match min_weight_size_n g u' v' x with
        | Some l => match acc with
                    | Some l' => if lt_weight_b l l' then Some l else Some l'
                    | None => Some l
@@ -1622,12 +1141,13 @@ Proof.
                  | None => None
                  end
        end) None l') = Some l'' ->
-      path' g u' v' l'' /\ (forall x p, In x l' -> path' g u' v' p -> length p = x -> le_weight l'' p)). { intros l'. induction l'; intros; simpl in H0.
+      path' g u' v' l'' /\ (forall x p, In x l' -> path' g u' v' p -> length p = x -> le_weight l'' p)). 
+{ intros l'. induction l'; intros; simpl in H0.
   - inversion H0.
-  - destruct (min_weight_size_n u' v' a0) eqn : M.
+  - destruct (min_weight_size_n g u' v' a0) eqn : M.
     + destruct (fold_right
              (fun (x : nat) (acc : option (list Node)) =>
-              match min_weight_size_n u' v' x with
+              match min_weight_size_n g u' v' x with
               | Some l0 =>
                   match acc with
                   | Some l' => if lt_weight_b l0 l' then Some l0 else Some l'
@@ -1654,11 +1174,11 @@ Proof.
       intros. subst. simpl in H4. destruct H4.
       apply H3. split. assumption. symmetry. assumption. apply F in H2.
       unfold min_weight_size_n in H2. rewrite min_list_empty in H2.
-      pose proof (paths_of_length_appear u' v' (length p) p). rewrite H2 in H4.
+      pose proof (paths_of_length_appear g u' v' (length p) p). rewrite H2 in H4.
       simpl in H4. exfalso. apply H4. split. assumption. reflexivity.
     + destruct (fold_right
          (fun (x : nat) (acc : option (list Node)) =>
-          match min_weight_size_n u' v' x with
+          match min_weight_size_n g u' v' x with
           | Some l =>
               match acc with
               | Some l' => if lt_weight_b l l' then Some l else Some l'
@@ -1672,7 +1192,7 @@ Proof.
       * apply IHl' in F. inversion H0; subst. destruct_all. split. assumption.
         intros. simpl in H3. destruct H3. subst. unfold min_weight_size_n in M.
         rewrite min_list_empty in M. exfalso. 
-        pose proof (paths_of_length_appear u' v' (length p) p). rewrite M in H3.
+        pose proof (paths_of_length_appear g u' v' (length p) p). rewrite M in H3.
         simpl in H3. apply H3. split. assumption. reflexivity. eapply H2. apply H3.
         assumption. assumption.
       * inversion H0. }
@@ -1685,7 +1205,7 @@ Proof.
   assumption.
 Qed.
 
-(*2 other lemmas that are good to know - and actually let me use this information in proofs*)
+(*If there is a path between u and v, there is a shortest path between u and v*)
 Lemma path_implies_shortest: forall u v l,
   path' g u v l ->
   exists l', shortest_wpath u v l'.
@@ -1695,14 +1215,7 @@ Proof.
   - rewrite find_shortest_wpath_none in D. specialize (D l). contradiction.
 Qed.
 
-Lemma path'_decidable: forall u v,
-  {exists l, path' g u v l} + {~exists l, path' g u v l}.
-Proof.
-  intros. destruct (find_shortest_wpath u v) eqn : D.
-  - left. exists l. apply find_shortest_wpath_correct in D. apply D.
-  - right. intro. destruct H. rewrite find_shortest_wpath_none in D. specialize (D x). contradiction.
-Qed.
-
+(*Any path with the same weight as a shortest path is also a shortest path*)
 Lemma shortest_wpath_same_weight: forall u v l l',
   shortest_wpath u v l ->
   path' g u v l' ->
@@ -1714,6 +1227,7 @@ Proof.
   apply H1. apply H3. assumption.
 Qed. 
 
+(*The shortest path from a vertex to itself is the trivial path*)
 Lemma shortest_path_refl: forall v,
   vIn g v = true ->
   shortest_wpath v v (v :: nil).
@@ -1734,7 +1248,7 @@ Definition sp_distance (g: gr a b) (o : option (list Node)) : option b :=
   | Some l => path_cost g l
   end.
 
-(*[sp_distance] unique*)
+(*[Any two shortest paths have the same weight*)
 Lemma sp_distance_unique: forall u v l1 l2,
   shortest_wpath u v l1 ->
   shortest_wpath u v l2 ->
@@ -1761,29 +1275,21 @@ Proof.
     order b.
 Qed.
 
-Lemma path_start: forall u v l,
-  path' g u v l -> exists l1, l = l1 ++ (u :: nil).
-Proof.
-  intros. induction H.
-  - exists nil. reflexivity.
-  - specialize (IHpath' Hsimple HNonneg). destruct_all. exists (v :: x). simpl. rewrite H1. reflexivity.
-Qed.
-
-(*Lemma 24.1 in CLRS*)
+(*Lemma 24.1 in CLRS - subpaths of shortest paths are also shortest paths*)
 Lemma shortest_path_subpath: forall u v v' l1 l2,
   shortest_wpath u v (l1 ++ v' :: l2) ->
   shortest_wpath u v' (v' :: l2).
 Proof.
-  intros. unfold shortest_wpath in *. destruct_all. split. apply path_app' in H. apply H.
+  intros. unfold shortest_wpath in *. destruct_all. split. apply path_app in H. apply H.
   intros. pose proof (lt_weight_total (v' :: l2) l'). unfold le_weight.
   destruct H2. simplify'. destruct H2. simplify'. destruct l'. inversion H1.
   assert (n = v'). rewrite path'_WPath in H1. destruct H1. eapply hd_path in H1. subst. reflexivity.
   subst. 
-  assert (path' g u v (l1 ++ v' :: l')). apply path_app' in H. rewrite path_app'. split.
+  assert (path' g u v (l1 ++ v' :: l')). apply path_app in H. rewrite path_app. split.
   apply H. assumption. apply H0 in H3.
   assert (exists w, path_cost g (l1 ++ v' :: l2) = Some w). apply path_cost_path'. exists u. exists v.
   assumption. assert (exists w, path_cost g (l1 ++ v' :: l') = Some w). apply path_cost_path'.
-  exists u. exists v. apply path_app' in H. apply path_app'. split. apply H. assumption.
+  exists u. exists v. apply path_app in H. apply path_app. split. apply H. assumption.
   destruct H4 as [w1]. destruct H5 as [w2].
   assert (path_cost g (l1 ++ v' :: l2) == Some w1 = true). rewrite H4. 
   rewrite simpl_option_some_eq. destruct HEqLaw as [E1 E2 E3]. apply E1.
